\documentclass[12pt]{article}
\thispagestyle{empty}

\begin{document}

\begin{eqnarray*}
  E & = & \frac{1}{2} \sum_i \sum_{j \neq i} V_{ij} \\
  V_{ij} & = & e^{-\lambda(r_{ij} -z_0}) \left[ C + f(\rho_{ij}) + f(\rho_{ji}) \right] - A \left( \frac{r_{ij}}{z_0}\right)^{-6} + A \left( \frac{\textrm{cutoff}}{z_0}\right)^{-6} \\
  \rho_{ij}^2 = \rho_{ji}^2 & = &  x_{ij}^2 + y_{ij}^2 ~\hspace{2cm} (\mathbf{n_i}\equiv\hat \mathbf{z})\\
  f(\rho) & = &  e^{-(\rho/\delta)^2} \sum_{n=0}^2 C_{2n} \left( \rho/\delta \right) ^{2n}
\end{eqnarray*}

\end{document}
