\documentclass[12pt]{article}

\begin{document}

$$
  q_i^C = \sum_{j \ne i} k_{ij} \omega_{CT}(r_{ij}) \left( \frac{1}{T_i} - \frac{1}{T_j} \right),
$$  
  
$$
  q_i^V = \frac{1}{2 C_v}\sum_{j \ne i}{ \left\{ \omega_D(r_{ij})\left[\gamma_{ij} \left( \mathbf{e}_{ij} \cdot \mathbf{v}_{ij} \right)^2 - \frac{\left( \sigma _{ij} \right)^2}{m}\right] - \sigma _{ij} \omega_R(r_{ij})\left( \mathbf{e}_{ij} \cdot \mathbf{v}_{ij} \right){\xi_{ij}} \right\} },
$$  

$$
  q_i^R = \sum_{j \ne i} \beta _{ij} \omega_{RT}(r_{ij}) d {t^{ - 1/2}} \xi_{ij}^e,
$$

$$
  \omega_{CT}(r)=\omega_{RT}^2(r)=\left(1-r/r_{ct}\right)^{s_T},
$$

$$
  k_{ij}=C_v^2\kappa(T_i + T_j)^2/4k_B,
$$

$$
  \beta_{ij}^2=2k_Bk_{ij},
$$

\end{document}
